Foundation/Modal/Neighborhood/AxiomM.lean
@@ -7,11 +7,11 @@ open Formula.Neighborhood
 variable {F : Frame}
 
 class Frame.IsMonotonic (F : Frame) : Prop where
-  mono : ∀ X Y : Set F, ℬ (X ∩ Y) ⊆ ℬ X ∩ ℬ Y
+  mono : ∀ X Y : Set F, F.box (X ∩ Y) ⊆ F.box X ∩ F.box Y
 
-lemma Frame.mono [Frame.IsMonotonic F] {X Y : Set F} : ℬ (X ∩ Y) ⊆ ℬ X ∩ ℬ Y := by apply IsMonotonic.mono
+lemma Frame.mono [Frame.IsMonotonic F] {X Y : Set F} : F.box (X ∩ Y) ⊆ F.box X ∩ F.box Y := by apply IsMonotonic.mono
 
-lemma Frame.mono' [Frame.IsMonotonic F] {X Y : Set F} : X ⊆ Y → ℬ X ⊆ ℬ Y := by
+lemma Frame.mono' [Frame.IsMonotonic F] {X Y : Set F} : X ⊆ Y → F.box X ⊆ F.box Y := by
   intro h x hX;
   apply @F.mono (X := X) (Y := Y) ?_ x ?_ |>.2;
   . assumption;
