Foundation/Modal/Neighborhood/Completeness.lean
@@ -93,36 +93,34 @@ structure CanonicalBox (𝓢 : S) where
   box : Set (MaximalConsistentSet 𝓢) → Set (MaximalConsistentSet 𝓢)
   canonicity : ∀ φ, box (proofset 𝓢 φ) = proofset 𝓢 (□φ)
 
+
+variable {𝓑 : CanonicalBox 𝓢}
+
+namespace CanonicalBox
+
 instance : CoeFun (CanonicalBox 𝓢) (fun _ => Set (MaximalConsistentSet 𝓢) → Set (MaximalConsistentSet 𝓢)) := ⟨CanonicalBox.box⟩
 
-def mkCanonicalFrame
-  (𝓢 : S) [Entailment.Consistent 𝓢] [Entailment.Cl 𝓢]
-  (box : CanonicalBox 𝓢)
-  : Frame := Frame.mk_ℬ (MaximalConsistentSet 𝓢) box
+protected def frame (𝓑 : CanonicalBox 𝓢) : Frame := Frame.mk_ℬ (MaximalConsistentSet 𝓢) 𝓑
 
-def mkCanonicalModel
-  (𝓢 : S) [Entailment.Consistent 𝓢] [Entailment.Cl 𝓢]
-  (box : CanonicalBox 𝓢)
-  : Model where
-  toFrame := mkCanonicalFrame 𝓢 box
+protected def model (𝓑 : CanonicalBox 𝓢) : Model where
+  toFrame := 𝓑.frame
   Val a := proofset 𝓢 (.atom a)
 
-@[simp] lemma mkCanonicalModel.eq_ℬ_self : (mkCanonicalModel 𝓢 box).box = box := by tauto;
+@[simp] lemma eq_model_box : 𝓑.model.box = 𝓑 := by tauto;
 
-lemma truthlemma : ↑(proofset 𝓢 φ) = ((mkCanonicalModel 𝓢 box).truthset φ) := by
+end CanonicalBox
+
+
+lemma truthlemma : ↑(proofset 𝓢 φ) = (𝓑.model.truthset φ) := by
   induction φ with
-  | hatom =>
-    simp [mkCanonicalModel]
-  | hfalsum =>
-    simp [mkCanonicalModel]
+  | hatom => simp [CanonicalBox.model]
+  | hfalsum => simp [CanonicalBox.model]
   | himp φ ψ ihφ ihψ =>
     simp_all [MaximalConsistentSet.proofset.eq_imp, ←ihφ, ←ihψ];
   | hbox φ ihφ =>
-    rw [Model.truthset.eq_box, ←ihφ, mkCanonicalModel.eq_ℬ_self, (@box.canonicity φ)];
+    rw [Model.truthset.eq_box, ←ihφ, CanonicalBox.eq_model_box, (@𝓑.canonicity φ)];
 
-lemma complete_of_canonical_frame
-  (C : FrameClass) (box)
-  (hC : (mkCanonicalFrame 𝓢 box) ∈ C)
+lemma complete_of_canonical_frame (C : FrameClass) (𝓑 : CanonicalBox 𝓢) (hC : 𝓑.frame ∈ C)
   : LO.Complete 𝓢 C := by
   constructor;
   intro φ;
@@ -131,7 +129,7 @@ lemma complete_of_canonical_frame
   have := FormulaSet.unprovable_iff_singleton_neg_consistent.mpr hφ;
   obtain ⟨Γ, hΓ⟩ := lindenbaum this;
   apply not_validOnFrameClass_of_exists_model_world;
-  use (mkCanonicalModel 𝓢 box), Γ;
+  use 𝓑.model, Γ;
   constructor;
   . assumption;
   . simp only [Semantics.Realize, Satisfies, ←truthlemma];
@@ -139,8 +137,10 @@ lemma complete_of_canonical_frame
     apply hΓ;
     tauto;
 
+
+
 open Classical in
-def minimal_canonical_box (𝓢 : S) [Entailment.E 𝓢] : CanonicalBox 𝓢 where
+protected abbrev CanonicalBox.minimal (𝓢 : S) [Entailment.E 𝓢] : CanonicalBox 𝓢 where
   box Γ := if h : ∃ φ, Γ = (proofset 𝓢 φ) then (proofset 𝓢 (□(h.choose))) else ∅
   canonicity := by
     intro φ;
@@ -150,25 +150,28 @@ def minimal_canonical_box (𝓢 : S) [Entailment.E 𝓢] : CanonicalBox 𝓢 whe
       apply h.choose_spec.symm;
     . tauto;
 
-namespace minimal_canonical_box
+namespace CanonicalBox.minimal
 
 variable {𝓢 : S} [Entailment.E 𝓢] [Consistent 𝓢]
 
-lemma exists_box (X) (Γ : (mkCanonicalFrame 𝓢 (minimal_canonical_box 𝓢)).World) (hΓ : Γ ∈ ℬ X)
-  : ∃ φ, X = proofset 𝓢 φ ∧ ℬ X = proofset 𝓢 (□φ)
+lemma exists_box (X) (Γ : (CanonicalBox.minimal 𝓢).model.World) (hΓ : Γ ∈ Frame.box _ X)
+  : ∃ φ, X = proofset 𝓢 φ ∧ Frame.box _ X = proofset 𝓢 (□φ)
   := by
-    simp [mkCanonicalFrame, Frame.mk_ℬ, minimal_canonical_box] at hΓ;
+    simp only [
+      CanonicalBox.minimal, CanonicalBox.model, CanonicalBox.frame, Frame.mk_ℬ, Frame.box,
+      Set.mem_setOf_eq, Set.setOf_mem_eq
+    ] at hΓ;
     split at hΓ;
     . rename_i h;
       obtain ⟨φ, hφ⟩ := h;
       use φ;
       constructor;
       . assumption;
-      . convert minimal_canonical_box 𝓢 |>.canonicity φ;
+      . convert CanonicalBox.minimal 𝓢 |>.canonicity φ;
     . contradiction;
 
-lemma exists_dia (X) (Γ : (mkCanonicalFrame 𝓢 (minimal_canonical_box 𝓢)).World) (hΓ : Γ ∈ ℬ X)
-  : ∃ φ, X = proofset 𝓢 φ ∧ 𝒟 X = proofset 𝓢 (◇φ)
+lemma exists_dia (X) (Γ : (CanonicalBox.minimal 𝓢).model.World) (hΓ : Γ ∈ Frame.box _ X)
+  : ∃ φ, X = proofset 𝓢 φ ∧ Frame.dia _ X = proofset 𝓢 (◇φ)
   := by
     obtain ⟨φ, hφ, hΓ⟩ := exists_box X Γ hΓ;
     use φ;
@@ -177,8 +180,9 @@ lemma exists_dia (X) (Γ : (mkCanonicalFrame 𝓢 (minimal_canonical_box 𝓢)).
     . ext Γ;
       rw [(show ◇φ = ∼□(∼φ) by rfl)];
       simp only [
-        minimal_canonical_box, mkCanonicalFrame, Frame.mk_ℬ, Set.mem_compl_iff,
-        Set.mem_setOf_eq, proofset.eq_neg
+        CanonicalBox.minimal, CanonicalBox.model, CanonicalBox.frame, Frame.mk_ℬ,
+        Frame.dia, Frame.box, Set.mem_setOf_eq, Set.setOf_mem_eq, Set.mem_compl_iff,
+        proofset.eq_neg
       ];
       constructor;
       . intro h;
@@ -202,7 +206,7 @@ lemma exists_dia (X) (Γ : (mkCanonicalFrame 𝓢 (minimal_canonical_box 𝓢)).
           simp;
         . tauto;
 
-end minimal_canonical_box
+end CanonicalBox.minimal
 
 
 end Neighborhood
