Foundation/Modal/Neighborhood/Supplementation.lean
@@ -1,24 +1,60 @@
 import Foundation.Modal.Neighborhood.Basic
 import Foundation.Modal.Neighborhood.AxiomM
+import Foundation.Modal.Neighborhood.AxiomC
 import Foundation.Modal.Neighborhood.AxiomGeach
 
 namespace LO.Modal.Neighborhood
 
 variable {F : Frame}
 
-def Frame.Supplementation (F : Frame) : Frame := Frame.mk_ℬ F.World (λ X => (Set.sUnion { ℬ Y | Y ⊆ X }))
+def Frame.Supplementation (F : Frame) : Frame := Frame.mk_ℬ F.World (λ X => (Set.sUnion { F.box Y | Y ⊆ X }))
 
 local postfix:80 "♯" => Frame.Supplementation
 
-lemma wow {w : F♯.World} : w ∈ ℬ X ↔ ∃ Y ⊆ X, w ∈ F.box Y := by
-  simp only [Frame.Supplementation, Frame.box, Frame.mk_ℬ, Set.mem_sUnion, Set.mem_setOf_eq, exists_exists_and_eq_and]
+namespace Frame.Supplementation
+
+lemma iff_exists_subset {X : Set (F.World)} {w : F.World} : w ∈ F♯.box X ↔ ∃ Y ⊆ X, w ∈ F.box Y := by
+  simp [Frame.Supplementation, Frame.box, Frame.mk_ℬ, Set.mem_sUnion, Set.mem_setOf_eq, exists_exists_and_eq_and]
+
+lemma subset (X : Set (F.World)) : F.box X ⊆ F♯.box X := by
+  intro x;
+  simp [Frame.Supplementation, Frame.box, Frame.mk_ℬ];
+  tauto;
+
+lemma monotonic {X Y : Set (F.World)} (h : X ⊆ Y) : F♯.box X ⊆ F♯.box Y := by
+  intro x hX;
+  obtain ⟨X', hX', hX⟩ := iff_exists_subset.mp hX;
+  apply iff_exists_subset.mpr;
+  use X';
+  constructor;
+  . apply Set.Subset.trans hX' h;
+  . assumption;
+
+lemma monotonic_iterated {X Y : Set (F.World)} (h : X ⊆ Y) (n) : F♯.box^[n] X ⊆ F♯.box^[n] Y := by
+  induction n with
+  | zero => simpa;
+  | succ n ih =>
+    rw [Function.iterate_succ'];
+    apply monotonic;
+    apply ih;
+
+lemma itl_reduce : F♯♯.box X = F♯.box X := by
+  ext x;
+  simp only [Supplementation, mk_ℬ, Set.mem_setOf_eq, Set.mem_sUnion, exists_exists_and_eq_and]
+  constructor;
+  . rintro ⟨Y, RYX, Z, RZY, hZ⟩;
+    use Z;
+    constructor;
+    . tauto_set;
+    . assumption;
+  . tauto;
 
 instance : F♯.IsMonotonic := by
   constructor;
   rintro X Y x hx;
-  obtain ⟨W, hW₁, hW₂⟩ := wow.mp hx;
+  obtain ⟨W, hW₁, hW₂⟩ := iff_exists_subset.mp hx;
   constructor <;>
-  . apply wow.mpr;
+  . apply iff_exists_subset.mpr;
     use W;
     constructor;
     . tauto_set;
@@ -27,7 +63,7 @@ instance : F♯.IsMonotonic := by
 instance [F.IsReflexive] : F♯.IsReflexive := by
   constructor;
   intro X w hw;
-  replace ⟨Y, hY₁, hY₂⟩ := wow.mp hw;
+  replace ⟨Y, hY₁, hY₂⟩ := iff_exists_subset.mp hw;
   apply hY₁;
   apply F.refl;
   exact hY₂;
@@ -35,8 +71,23 @@ instance [F.IsReflexive] : F♯.IsReflexive := by
 instance [F.IsTransitive] : F♯.IsTransitive := by
   constructor;
   intro X w hw;
-  obtain ⟨Y, hY₁, hY₂⟩ := wow.mp hw;
-  have := F.trans hY₂;
-  sorry;
+  obtain ⟨Y, hYX, hY⟩ := iff_exists_subset.mp hw;
+  apply monotonic_iterated hYX 2
+  apply monotonic $ subset Y;
+  apply subset (F.box Y) $ F.trans hY;
+
+instance [F.IsRegular] : F♯.IsRegular := by
+  constructor;
+  rintro X Y w ⟨hX, hY⟩;
+  apply iff_exists_subset.mpr;
+  obtain ⟨X', _⟩ := iff_exists_subset.mp hX;
+  obtain ⟨Y', _⟩ := iff_exists_subset.mp hY;
+  use X' ∩ Y';
+  constructor;
+  . tauto_set;
+  . apply @Frame.regular F _ X' Y';
+    tauto;
+
+end Frame.Supplementation
 
 end LO.Modal.Neighborhood
